# Рекурсивное решение Веселовского
### Info type
6_Related_Works
### Keywords
#Литература2Веселовский, #магические квадраты, #литература, #Веселовский, #рекурсия
### Text
2. Другое решение от Аркадиуса было найдено раньше, а соотнести его с нашим исследованием будет сложнее, так как оно записывается рекурсивно:
Received December 20 and 22. 2019
One year after his above parametric solutions of 3x3 magic squares of 5 squared integers, one more squared integer! Arkadiusz Wesolowski found this marvelous parametric solution of 3x3 magic squares of 6 squared integers:
$$x = \frac{[(3 + \sqrt{3}) \cdot (2 + \sqrt{3}) + 1 + (3 - \sqrt{3}) \cdot (2 - \sqrt{3}) + 1]}{6}$$
$$y = \frac{[(3 + \sqrt{3}) \cdot (2 + \sqrt{3}) + (3 - \sqrt{3}) \cdot (2 - \sqrt{3})]}{6}$$
$$z = 2 \cdot \frac{[(1 + \frac{\sqrt{3}}{2}) + 1 - (1 - \frac{\sqrt{3}}{2}) + 1]}{\sqrt{3}}$$
$$
\begin{matrix}
(xy - z)^2 & (x + yz)^2 & x^2z^2 + y^2 \\
(xz - y)^2 & x^2 + y^2z^2 & (xy + z)^2 \\
(yz - x)^2 & (x^2 + y^2)(z^2 + 1) / 2 & (xz + y)^2
\end{matrix}
$$
The three first examples of 3x3 magic squares, constructed with n = 1 (-> (x, y, z) = (11, 3, 4)), n = 2 (-> (41, 11, 15)), and n = 3 (-> (153, 41, 56)):
$$
\begin{matrix}
29^2 & 47^2 & 265 \\
23^2 & 1105 & 41^2 \\
1945 & 12 & 37^2
\end{matrix}
$$
$$
\begin{matrix}
4362 & 6262 & 28906 \\
2062 & 203626 & 6042 \\
378346 & 1242 & 4662
\end{matrix}
$$
$$
\begin{matrix}
62172 & 86092 & 5295025 \\
24492 & 39353665 & 85272 \\
73412305 & 21432 & 63292
\end{matrix}
$$
When n is an even positive number, we can prove that the cells in red can't be squared integers. His quick search of odd n <= 2*10^5 didn't produce 3x3 magic squares with seven, eight, or nine square numbers. But maybe a larger odd n?
This was not given by Arkadiusz, but x, y, z can be easily computed with these recurrence formulas:
$$
\begin{cases}
x(0) = 3 \\
y(0) = 1 \\
z(0) = 1
\end{cases}
$$
$$
\begin{cases}
x(n) = 3x(n - 1) + 2z(n - 1) \\
y(n) = x(n - 1) \\
z(n) = x(n - 1) + z(n - 1)
\end{cases}
$$
Пусть E, X, Y — определяющие по нашей теории квадрат параметры. Заметим, что
$$E = \frac{(x^2 + y^2)(z^2 + 1)}{2}$$
$$Y = A - H = (xy - z)^2 - (yz - x)^2 = (x^2 - z^2)(y^2 - 1)$$
$$Y = F - A = (xz - y)^2 - (xy - z)^2 = (x^2 - y^2)(z^2 - 1)$$
$$X = \frac{(xy + z)^2 - (xy - z)^2}{2} = 4xyz$$
$$Y = (9x^2 + 12xz + 4z^2)$$
Теперь выпишем первые несколько значений, чтобы узреть красоту взаимосвязи:
$$
\begin{matrix}
x & y & z & E & X & Y \\
3 & 1 & 1 & 10 & 6 & 0 = 4f(1, 1) = 4f(2, 0) \\
11 & 3 & 4 & 1105 & 264 & 840 = 4f(5, 2) = 4f(6, 1) \\
41 & 11 & 15 & 203626 & 13530 & 174720 = 4f(20, 6) = 4f(21, 5) \\
153 & 41 & 56 & 39353665 & 702576 & 34058640 = 4f(76, 21) = 4f(77, 20) \\
571 & 153 & 209 & 15264674900 & 36517734 & 6609482880 = 4f(285, 77) = 4f(286, 76)
\end{matrix}
$$
Заметим, что $Y = 4f(\frac{x - 1}{2}, \frac{y + 1}{2}) = 4f(\frac{x + 1}{2}, \frac{y - 1}{2})$ и докажем. Но прежде докажем, что $2z = x - y$. Для начального случая верно: $2z_0 = 2 = 3 - 1 = x_0 - y_0$. Для последующих также верно: $2z_{n + 1} = 2x_n + 2z_n = (3x_n + 2z_n) - x_n = x_{n + 1} - y_{n + 1}$.
$$z_{n + 1} = \frac{x_{n + 1} - y_{n + 1}}{2}$$
Теперь, избавившись от 2, можем переписать выражения выше: